added the following flags
main.native -no-gvn input.bc ;; null pass
main.native -disable-load-elim input.bc ;; no load elim
main.native -disable-pre input.bc ;; no pre
main.native -disable-both input.bc ;; only do CSE/DCE
main.native input.bc ;; CSE + PRE + LoadElim + DCE

Some proofs of dom-tree construction



git-svn-id: https://webdav.seas.upenn.edu/svn/sol/vol@3379 eef5ea85-cc2e-0410-bd84-0fae1f012da8

src/Transforms/main.ml
@@ -42,5 +42,13 @@ let () = match Sys.argv with
        Globalstates.debug := true; main in_filename
   | [| _; "-no-gvn" ; in_filename |] -> 
        nogvn := true; main in_filename
+  | [| _; "-disable-pre" ; in_filename |] -> 
+      Globalstates.does_pre := false; main in_filename
+  | [| _; "-disable-load-elim" ; in_filename |] -> 
+      Globalstates.does_load_elim := false; main in_filename
+  | [| _; "-disable-both" ; in_filename |] -> 
+      Globalstates.does_load_elim := false; 
+      Globalstates.does_pre := false; 
+      main in_filename
   | [| _; in_filename |] -> main in_filename
   | _ -> main "input.bc"
