src/Transforms/dtree.v
@@ -149,7 +149,7 @@ match dt with
 end.
 
 Inductive WF_dtree (f:fdef) : DTree -> Prop :=
-| WDT_note : forall (l0:l) (dts0:DTrees),
+| WDT_node : forall (l0:l) (dts0:DTrees),
              reachable f l0 ->
              l0 `notin` dtrees_dom dts0 ->
              WF_dtrees f l0 dts0 ->
@@ -188,6 +188,253 @@ match AMap.get l0 res with
 | l1::dts0 => find_idom_aux res l1 dts0
 | _ => None
 end.
+
+Require Import Trees.
+
+Fixpoint dtree_insert dt parent child : option DTree :=
+match dt with
+| DT_node l0 dts0 => 
+    if (id_dec parent l0) then 
+      Some (DT_node l0 (DT_cons (DT_node child DT_nil) dts0))
+    else 
+      match dtrees_insert dts0 parent child with
+      | Some dts1 => Some (DT_node l0 dts1)
+      | None => None
+      end
+end
+with dtrees_insert (dts: DTrees) parent child : option DTrees :=
+match dts with
+| DT_nil => Some DT_nil
+| DT_cons dt0 dts0 => 
+    match dtree_insert dt0 parent child, dtrees_insert dts0 parent child with
+    | Some dt1, Some dts1 => Some (DT_cons dt1 dts1)
+    | _, _ => None
+    end
+end.
+
+Fixpoint tree2dtree vs es (tree: Tree vs es) : option DTree :=
+match tree with
+| T_root (index le) => Some (DT_node le DT_nil)
+| T_leaf vs' es' t' (index child) (index parent) _ _ => 
+    match tree2dtree vs' es' t' with
+    | Some dt' => dtree_insert dt' parent child
+    | _ => None
+    end
+| T_eq vs1 vs2 es1 es2 _ _ t1 => tree2dtree vs1 es1 t1
+end.
+
+Definition PreDTree := list (l * l).
+
+Definition getEntryLabel (f:fdef) : option l :=
+match f with
+| fdef_intro _ ((block_intro l0 _ _ _)::_) => Some l0
+| _ => None
+end.
+
+Fixpoint cdom (pdt: PreDTree) : atoms :=
+match pdt with
+| nil => empty
+| (_,l2)::pdt' => add l2 (cdom pdt')
+end.
+
+Inductive WF_pre_dtree (f:fdef) : PreDTree -> Type :=
+| WPDT_entry : forall entry child,
+    getEntryLabel f = Some entry ->
+    imm_domination f entry child -> 
+    WF_pre_dtree f ((entry, child)::nil)
+| WPDT_cons : forall parent child pdt,
+    WF_pre_dtree f pdt ->
+    reachable f parent ->
+    imm_domination f parent child -> 
+    child `notin` dom pdt `union` cdom pdt ->
+    (parent `in` dom pdt \/ exists ancestor, In (ancestor, parent) pdt) -> 
+    WF_pre_dtree f ((parent, child) :: pdt).
+
+Definition arcs_of_pre_dtree (pdt: PreDTree) : A_set :=
+fun arc =>
+  match arc with
+  | A_ends (index parent) (index child) => 
+      In (parent, child) pdt \/ In (child, parent) pdt
+  end.
+
+Definition vertexes_of_pre_dtree (pdt: PreDTree) : V_set :=
+fun v =>
+  match v with
+  | index n => exists n', In (n, n') pdt \/ In (n', n) pdt
+  end.
+
+Lemma In_vertexes_of_pre_dtree: forall l1 l2 pdt,
+  In (l1, l2) pdt -> vertexes_of_pre_dtree pdt (index l2).
+Proof.
+  induction pdt; simpl; intros.
+    inv H.
+    exists l1.
+    destruct H as [H | H]; subst; auto.
+Qed.
+
+Lemma In_vertexes_of_pre_dtree': forall l1 l2 pdt,
+  In (l1, l2) pdt -> vertexes_of_pre_dtree pdt (index l1).
+Proof.
+  induction pdt; simpl; intros.
+    inv H.
+    exists l2.
+    destruct H as [H | H]; subst; auto.
+Qed.
+
+Lemma InDom_vertexes_of_pre_dtree: forall l1 pdt,
+  l1 `in` dom pdt -> vertexes_of_pre_dtree pdt (index l1).
+Proof.
+  induction pdt; simpl; intros.
+    fsetdec.
+
+    destruct a.
+    assert (l1 = a \/ l1 `in` dom pdt) as Hin.
+      fsetdec.
+    destruct Hin as [Hin | Hin]; subst.
+      exists l0. auto.
+      apply IHpdt in Hin. simpl in Hin.
+      destruct Hin as [n' [Hin | Hin]]; exists n'; auto.
+Qed.
+
+Lemma Notin_vertexes_of_pre_dtree: forall child pdt
+  (n : child `notin` dom pdt `union` cdom pdt),
+  ~ vertexes_of_pre_dtree pdt (index child).
+Proof.
+  induction pdt; simpl; intros.
+    intro J. destruct J as [_ [J | J]]; inv J.
+
+    intro J. 
+    destruct J as [n' [J | J]].
+      destruct J as [J | J]; subst.
+        fsetdec.
+        
+        destruct a.    
+        apply In_vertexes_of_pre_dtree' in J.
+        revert J. 
+        apply IHpdt; auto.
+      destruct J as [J | J]; subst.
+        fsetdec.
+
+        destruct a.    
+        apply In_vertexes_of_pre_dtree in J.
+        revert J. 
+        apply IHpdt; auto.
+Qed.
+
+Lemma In_arcs_of_pre_dtree: forall a a0 pdt,
+  In (a, a0) pdt ->
+  Ensembles.In Arc (arcs_of_pre_dtree pdt) (A_ends (index a) (index a0)).
+Proof.
+  induction pdt; simpl; intros.
+    inv H.
+
+    unfold Ensembles.In. simpl.
+    destruct H as [H | H]; subst; auto.
+Qed.
+
+Lemma In_arcs_of_pre_dtree': forall a a0 pdt,
+  In (a0, a) pdt ->
+  Ensembles.In Arc (arcs_of_pre_dtree pdt) (A_ends (index a) (index a0)).
+Proof.
+  induction pdt; simpl; intros.
+    inv H.
+
+    unfold Ensembles.In. simpl.
+    destruct H as [H | H]; subst; auto.
+Qed.
+
+Lemma WF_pre_dtree_isa_tree: forall f pdt, 
+  WF_pre_dtree f pdt -> 
+  Tree (vertexes_of_pre_dtree pdt) (arcs_of_pre_dtree pdt).
+Proof.
+  intros f pdt Hwf.
+  induction Hwf.
+    apply T_eq with 
+      (v:=V_union (V_single (index child)) (V_single (index entry)))
+      (a:=A_union (E_set (index entry) (index child)) A_empty).
+      apply U_set_eq.
+        intros x.
+        split; intro J.
+          inv J; inv H; simpl.
+            exists entry. auto.
+            exists child. auto.
+          destruct x; simpl in J.
+          destruct J as [n' [J | J]].
+            destruct J as [J | J]; inv J. 
+            apply In_right. apply In_single; auto.
+
+            destruct J as [J | J]; inv J. 
+            apply In_left. apply In_single; auto.
+      apply A_set_eq.
+        intros x.
+        split; intro J.
+          inv J; inv H; simpl; auto.
+
+          destruct x as [[] []]; simpl in J.
+          destruct J as [J | J].
+            destruct J as [J | J]; inv J. 
+            apply In_left. apply E_right.
+
+            destruct J as [J | J]; inv J. 
+            apply In_left. apply E_left.
+      apply T_leaf.
+        apply T_root.
+        apply In_single; auto.
+
+        intro J. inv J. 
+        unfold imm_domination, strict_domination in i0.
+        destruct i0 as [[_ J] _]; auto.
+
+    apply T_eq with 
+      (v:=V_union (V_single (index child)) (vertexes_of_pre_dtree pdt))
+      (a:=A_union (E_set (index parent) (index child)) (arcs_of_pre_dtree pdt)).
+      apply U_set_eq.
+        intros [v].
+        split; intro J.
+          inv J; inv H.
+            exists parent. simpl. auto.
+
+            destruct H0 as [H0 | H0].
+              eapply In_vertexes_of_pre_dtree'; simpl; eauto.
+              eapply In_vertexes_of_pre_dtree; simpl; eauto.
+
+          destruct J as [n' [J | J]]; simpl in J.
+            apply In_right. 
+            destruct J as [J | J].
+              inv J. 
+              clear - o. destruct o as [o | [anc e]].
+                eapply InDom_vertexes_of_pre_dtree; eauto.
+                apply In_vertexes_of_pre_dtree in e; auto.
+
+              apply In_vertexes_of_pre_dtree' in J; auto.
+            destruct J as [J | J].
+              inv J. 
+              apply In_left. apply In_single.
+
+              apply In_right. 
+              apply In_vertexes_of_pre_dtree in J; auto.
+      apply A_set_eq.
+        intros [v1 v2]. destruct v1, v2.
+        split; intro J.
+          inv J; inv H; simpl; auto.
+
+          inv J.
+            simpl in H. 
+            destruct H as [H | H].
+              inv H.
+              apply In_left. apply E_right.
+              apply In_right. apply In_arcs_of_pre_dtree; auto.
+            simpl in H. 
+            destruct H as [H | H].
+              inv H.
+              apply In_left. apply E_left.
+              apply In_right. apply In_arcs_of_pre_dtree'; auto.
+      apply T_leaf; auto.
+        clear - o. destruct o as [o | [anc e]].
+          eapply InDom_vertexes_of_pre_dtree; eauto.
+          apply In_vertexes_of_pre_dtree in e; auto.
+        apply Notin_vertexes_of_pre_dtree; auto.
+Qed.
 
 Fixpoint find_children (res: AMap.t (set l)) (root:l) 
   (others:set l) (acc:list l): option (list l) :=
@@ -310,8 +557,114 @@ Proof.
     apply incl_refl.
 Qed.
 
-Program Fixpoint create_dtree_aux (res: AMap.t (set l)) 
-  (root:l) (others:set l) {measure (List.length others)}
+Fixpoint compute_idoms (res: AMap.t (set l)) (bd: list l) (acc: list (l * l)) :
+  list (l * l) :=
+match bd with
+| nil => acc
+| l0 :: bd' =>
+    match find_idom res l0 with
+    | None => compute_idoms res bd' acc
+    | Some l1 => compute_idoms res bd' ((l1,l0)::acc)
+    end
+end.
+
+Fixpoint find_next_child (idoms: list (l * l)) (parent: l) (others:set l) 
+  : option l :=
+match idoms with
+| nil => None
+| (l1, l2)::idoms' =>
+    if (l_dec l1 parent) then 
+      if (in_dec l_dec l2 others) then Some l2
+      else find_next_child idoms' parent others
+    else find_next_child idoms' parent others
+end.
+
+Fixpoint find_next_sub_pre_dtree_aux (idoms: list (l * l)) (pdt0 pdt:PreDTree) 
+  (others:set l) : option (PreDTree * set l) :=
+match pdt with
+| nil => None
+| (p, ch)::pdt' => 
+    match find_next_child idoms ch others with
+    | None => 
+        match find_next_child idoms p others with
+        | None => 
+            find_next_sub_pre_dtree_aux idoms pdt0 pdt' others
+        | Some ch' =>
+            Some ((p, ch')::pdt0, List.remove l_dec ch' others)
+        end
+    | Some ch' => Some ((ch, ch')::pdt0, List.remove l_dec ch' others)
+    end
+end.
+
+Definition find_next_sub_pre_dtree (idoms: list (l * l)) (pdt:PreDTree) 
+  (others:set l) : option (PreDTree * set l) :=
+find_next_sub_pre_dtree_aux idoms pdt pdt others.
+
+Lemma find_next_child_inv : forall idoms l1 others l2,
+  find_next_child idoms l1 others = ret l2 ->
+  In l2 others /\ In (l1, l2) idoms.
+Proof.
+  induction idoms; simpl; intros.
+    inv H.
+
+    destruct a.
+    destruct (l_dec l0 l1); subst.
+      destruct (in_dec l_dec l3 others).
+        inv H. auto.
+        apply IHidoms in H. destruct H. split; auto.
+      apply IHidoms in H. destruct H. split; auto.
+Qed.       
+
+Lemma find_next_sub_pre_dtree_aux_length: forall idoms pdt0 acc others acc' others',
+  find_next_sub_pre_dtree_aux idoms pdt0 acc others = ret (acc', others') ->
+  (length others' < length others)%nat.
+Proof.
+  induction acc; simpl; intros.
+    inv H. 
+
+    destruct a.
+    remember (find_next_child idoms l1 others) as R.
+    destruct R.
+      inv H.
+      symmetry in HeqR.
+      apply find_next_child_inv in HeqR.
+      destruct HeqR.
+      apply remove_in_length; auto.
+
+      remember (find_next_child idoms l0 others) as R.
+      destruct R; eauto.
+        inv H.
+        symmetry in HeqR0.
+        apply find_next_child_inv in HeqR0.
+        destruct HeqR0.
+        apply remove_in_length; auto.
+Qed.
+
+Lemma find_next_sub_pre_dtree_length: forall idoms acc others acc' others',
+  find_next_sub_pre_dtree idoms acc others = ret (acc', others') ->
+  (length others' < length others)%nat.
+Proof.
+  intros.
+  unfold find_next_sub_pre_dtree in H.
+  apply find_next_sub_pre_dtree_aux_length in H; auto.
+Qed.
+
+Program Fixpoint create_pre_dtree_aux (others:set l) (idoms: list (l * l)) 
+  (acc:PreDTree) {measure (List.length others)} : option PreDTree :=
+match others with
+| nil => Some acc
+| _ =>
+   match find_next_sub_pre_dtree idoms acc others with
+   | None => None
+   | Some (acc', others') => create_pre_dtree_aux others' idoms acc'
+   end
+end.
+Next Obligation. 
+  eapply find_next_sub_pre_dtree_length; eauto.
+Qed.
+
+Program Fixpoint create_dtree_aux (others:set l) (res: AMap.t (set l)) 
+  (root:l) {measure (List.length others)}
   : option DTree :=
 match find_children res root others nil with
 | Some nil => Some (DT_node root DT_nil)
@@ -321,7 +674,7 @@ match find_children res root others nil with
     let op_dts0 :=
       (fold_left 
         (fun acc l1 => 
-         match acc, create_dtree_aux res l1 others' with
+         match acc, create_dtree_aux others' res l1 with
          | Some dts0, Some dt0 => Some (DT_cons dt0 dts0) 
          | _, _ => None
          end)
@@ -341,7 +694,6 @@ Next Obligation.
 Qed.
 Next Obligation. split; intros; congruence. Qed.
 
-
 Fixpoint dep_doms__nondep_doms_aux bd0 (res: AMap.t (Dominators.t bd0)) 
   bd (acc: AMap.t (set l)) : AMap.t (set l) :=
 match bd with
@@ -357,6 +709,469 @@ Definition dep_doms__nondep_doms bd (res: AMap.t (Dominators.t bd))
   : AMap.t (set l) :=
 dep_doms__nondep_doms_aux bd res bd (AMap.init nil).
 
+Fixpoint init_pre_dtree (idoms: list (l * l)) (root:l) (others:set l)
+  : option (PreDTree * list l) :=
+match idoms with 
+| nil => None
+| (p, ch)::idoms' => 
+    if (l_dec p root) then 
+      if (in_dec l_dec ch others) then 
+        Some ([(p, ch)], List.remove l_dec ch others)
+      else None
+    else init_pre_dtree idoms' root others
+end.
+
+Inductive WF_idoms f : list (l*l) -> Type :=
+| WF_idoms_nil : WF_idoms f nil 
+| WF_idoms_cons : forall l1 l2 idoms, 
+    imm_domination f l1 l2 -> WF_idoms f idoms ->
+    WF_idoms f ((l1,l2)::idoms)
+.
+
+Lemma WF_pre_dtree__reachable: forall f acc l1 l2,
+  WF_pre_dtree f acc ->
+  In (l1, l2) acc ->
+  reachable f l1 /\ reachable f l2.
+Admitted.
+
+Lemma find_next_child__imm_domination: forall f idoms (Hwfi: WF_idoms f idoms) 
+  l1 others l2,
+  find_next_child idoms l1 others = ret l2 ->
+  imm_domination f l1 l2.
+Proof.
+  induction idoms; simpl; intros.
+    inv H.
+
+    destruct a.
+    inv Hwfi.
+    destruct (l_dec l0 l1); subst; eauto.
+      destruct (in_dec l_dec l3 others); eauto.
+        inv H. auto.
+Qed.
+
+Lemma find_next_sub_pre_dtree_aux_wf_pre_dtree: 
+  forall f idoms (Hwfi: WF_idoms f idoms) acc prefix 
+    (Hwf:WF_pre_dtree f (prefix++acc)) others acc' others'
+  (Hdis: forall l0, 
+    In l0 others -> 
+    l0 `notin` dom (prefix++acc) `union` cdom (prefix++acc)),
+  find_next_sub_pre_dtree_aux idoms (prefix++acc) acc others = 
+    ret (acc', others') ->
+  WF_pre_dtree f acc'.
+Proof.
+  induction acc; simpl; intros.
+    congruence.
+
+    destruct a.
+    remember (find_next_child idoms l1 others) as R.
+    destruct R.
+      inv H.
+      apply WPDT_cons; auto.
+        apply WF_pre_dtree__reachable with (l1:=l0)(l2:=l1) in Hwf.
+          destruct Hwf; auto.
+          apply in_middle.
+        eapply find_next_child__imm_domination; eauto.
+
+        symmetry in HeqR.
+        apply find_next_child_inv in HeqR.
+        destruct HeqR as [J1 J2]. auto.
+
+        right.
+        exists l0. apply in_middle.
+
+      remember (find_next_child idoms l0 others) as R.
+      destruct R.
+        inv H.
+        apply WPDT_cons; auto.
+          apply WF_pre_dtree__reachable with (l1:=l0)(l2:=l1) in Hwf.
+            destruct Hwf; auto.
+            apply in_middle.
+          eapply find_next_child__imm_domination; eauto.
+
+          symmetry in HeqR0.
+          apply find_next_child_inv in HeqR0.
+          destruct HeqR0 as [J1 J2]. auto.
+          left. simpl_env. fsetdec.
+      rewrite_env ((prefix ++ [(l0, l1)]) ++ acc) in H.
+      apply IHacc in H; simpl_env; simpl; auto.
+Qed.
+
+Lemma find_next_sub_pre_dtree_wf_pre_dtree: 
+  forall f idoms (Hwfi: WF_idoms f idoms) pdt (Hwf:WF_pre_dtree f pdt) 
+    others pdt' others'
+  (Hdis: forall l0, 
+    In l0 others -> 
+    l0 `notin` dom pdt `union` cdom pdt),
+  find_next_sub_pre_dtree idoms pdt others = ret (pdt', others') ->
+  WF_pre_dtree f pdt'.
+Proof.
+  intros.
+  unfold find_next_sub_pre_dtree in H.
+  change pdt with (nil++pdt) in H, Hdis at 1.
+  eapply find_next_sub_pre_dtree_aux_wf_pre_dtree in H; eauto.
+Qed.
+
+Definition P_create_pre_dtree_aux__WF_pre_dtree (n:nat) :=
+  forall f idoms (Hwfi: WF_idoms f idoms) pdt0 others pdt
+  (Hdis: forall l0, 
+    In l0 others -> 
+    l0 `notin` dom pdt0 `union` cdom pdt0),
+  List.length others = n ->
+  WF_pre_dtree f pdt0 ->
+  create_pre_dtree_aux others idoms pdt0 = Some pdt ->
+  WF_pre_dtree f pdt.
+
+Require Import Program.
+
+Ltac simple_create_pre_dtree_aux :=
+  unfold create_pre_dtree_aux, create_pre_dtree_aux_func;
+  rewrite WfExtensionality.fix_sub_eq_ext;
+  repeat fold_sub create_pre_dtree_aux_func ; simpl proj1_sig;
+  simpl. 
+
+Lemma find_next_sub_pre_dtree_aux_inv: forall idoms pdt0 pdt others pdt' 
+  others',
+  find_next_sub_pre_dtree_aux idoms pdt0 pdt others = Some (pdt', others') ->
+  exists p, exists ch, 
+    pdt' = (p,ch)::pdt0 /\ others' = List.remove l_dec ch others /\
+    ((exists p', In (p', p) pdt) \/ (exists ch', In (p, ch') pdt)).
+Proof.
+  induction pdt; simpl; intros.
+    inv H.
+
+    destruct a.
+    remember (find_next_child idoms l1 others) as R.
+    destruct R.
+      inv H.
+      exists l1. exists l2. 
+      repeat split; auto.
+      left. exists l0. auto.
+
+      remember (find_next_child idoms l0 others) as R. 
+      destruct R.
+        inv H.
+        exists l0. exists l2. 
+        repeat split; auto.
+        right. exists l1. auto.
+       
+        apply IHpdt in H; auto.
+        destruct H as [p [ch [Heq1 [Heq2 [[p' J] | [ch' J]]]]]]; subst.
+          exists p. exists ch. 
+          repeat split; auto.
+          left. exists p'. auto.
+
+          exists p. exists ch. 
+          repeat split; auto.
+          right. exists ch'. auto.
+Qed.
+
+Lemma find_next_sub_pre_dtree_inv: forall idoms pdt others pdt' 
+  others',
+  find_next_sub_pre_dtree idoms pdt others = Some (pdt', others') ->
+  exists p, exists ch, 
+    pdt' = (p,ch)::pdt /\ others' = List.remove l_dec ch others /\
+    ((exists p', In (p', p) pdt) \/ (exists ch', In (p, ch') pdt)).
+Proof.
+  intros. unfold find_next_sub_pre_dtree in H.
+  apply find_next_sub_pre_dtree_aux_inv in H; auto.
+Qed.
+
+Lemma in_dom_cdom: forall p1 p2 pdt0,
+  In (p1, p2) pdt0 -> p2 `in` cdom pdt0 /\ p1 `in` dom pdt0.
+Proof.
+  induction pdt0; simpl; intros.
+    inv H.
+    destruct H as [H | H]; subst.
+      fsetdec.
+
+      destruct a.
+      apply IHpdt0 in H.
+      fsetdec.
+Qed.
+
+Lemma create_pre_dtree_aux__WF_pre_dtree_aux: forall n, 
+  P_create_pre_dtree_aux__WF_pre_dtree n.
+Proof.
+  intro n.
+  apply lt_wf_rec. clear n.
+  intros n IH.
+  unfold P_create_pre_dtree_aux__WF_pre_dtree in *.
+  intros f idoms Hwfi pdt0 others pdt Hdis Hlen Hwf.
+  destruct others as [|l1 others]; simple_create_pre_dtree_aux.
+    intro J. inv J; auto.
+
+    remember (find_next_sub_pre_dtree idoms pdt0 (l1 :: others)) as R.
+    destruct R as [[acc' others']|].
+      repeat fold_sub create_pre_dtree_aux_func ; simpl proj1_sig.
+      fold (create_pre_dtree_aux others' idoms acc').
+      intro J. subst.
+      apply IH with (m:=length others') (f:=f) in J; auto.
+        eapply find_next_sub_pre_dtree_length; eauto.
+
+        symmetry in HeqR.
+        apply find_next_sub_pre_dtree_inv in HeqR.
+        destruct HeqR as [p [ch [Heq [J1 [[p' J2] | [ch' J2]]]]]]; subst.
+          intros l0 Hin.
+          simpl.
+          assert (l0 <> ch) as Hneq.
+            assert (J':=@remove_In _ l_dec (l1 :: others) ch).
+            destruct (l_dec l0 ch); subst; auto.
+          assert (In l0 (l1::others)) as Hin'.
+            apply remove_neq_in' in Hin; auto.
+          apply Hdis in Hin'.
+          apply in_dom_cdom in J2.
+          destruct J2 as [J1 J2].
+          assert (l0 <> p) as Hneq'.
+            destruct (l_dec l0 p); subst; auto.
+          fsetdec.
+ 
+          intros l0 Hin.
+          simpl.
+          assert (l0 <> ch) as Hneq.
+            assert (J':=@remove_In _ l_dec (l1 :: others) ch).
+            destruct (l_dec l0 ch); subst; auto.
+          assert (In l0 (l1::others)) as Hin'.
+            apply remove_neq_in' in Hin; auto.
+          apply Hdis in Hin'.
+          apply in_dom_cdom in J2.
+          destruct J2 as [J1 J2].
+          assert (l0 <> p) as Hneq'.
+            destruct (l_dec l0 p); subst; auto.
+          fsetdec.
+        eapply find_next_sub_pre_dtree_wf_pre_dtree; eauto.
+      intro J. inv J.
+Qed.
+
+Lemma create_pre_dtree_aux__WF_pre_dtree : forall f idoms 
+  (Hwfi: WF_idoms f idoms) pdt0 others pdt
+  (Hdis: forall l0, 
+    In l0 others -> 
+    l0 `notin` dom pdt0 `union` cdom pdt0),
+  WF_pre_dtree f pdt0 ->
+  create_pre_dtree_aux others idoms pdt0 = Some pdt ->
+  WF_pre_dtree f pdt.
+Proof.
+  intros.
+  assert (J:=@create_pre_dtree_aux__WF_pre_dtree_aux (List.length others)).
+  unfold P_create_pre_dtree_aux__WF_pre_dtree in J. eauto.
+Qed.
+
+Lemma init_pre_dtree__WF_pre_dtree : forall f root 
+  (Hentry:getEntryLabel f = Some root) idoms 
+  (Hwfi: WF_idoms f idoms) others pdt0 others0,
+  init_pre_dtree idoms root others = Some (pdt0, others0) ->
+  WF_pre_dtree f pdt0.
+Proof.
+  induction idoms; simpl; intros.
+    inv H.
+
+    destruct a.
+    inv Hwfi.
+    destruct (l_dec l0 root); subst; eauto.
+      destruct (in_dec l_dec l1 others); inv H.
+      apply WPDT_entry; auto.
+Qed.
+
+Lemma init_pre_dtree__disjoint: forall root idoms others pdt0 others0,
+  init_pre_dtree idoms root others = ret (pdt0, others0) ->
+  ~ In root others ->
+  forall l0 : atom, In l0 others0 -> l0 `notin` union (dom pdt0) (cdom pdt0).
+Proof.
+  induction idoms; simpl; intros.
+    inv H.
+
+    destruct a.
+    destruct (l_dec l1 root); subst.
+      destruct (in_dec l_dec l2 others); inv H.
+        simpl.
+        assert (l0 <> l2) as Hneq.
+          assert (J':=@remove_In _ l_dec others l2).
+          destruct (l_dec l0 l2); subst; auto.
+        assert (In l0 others) as Hin'.
+          apply remove_neq_in' in H1; auto.
+        assert (l0 <> root) as Hneq'.
+          destruct (l_dec l0 root); subst; auto.
+        fsetdec.
+
+      eapply IHidoms in H; eauto.        
+Qed.
+
+Lemma compute_idoms__WF_idoms_aux: forall f rd idoms acc,
+  reachablity_analysis f = Some rd ->
+  WF_idoms f acc ->
+  compute_idoms (dep_doms__nondep_doms (bound_fdef f) (dom_analyze f)) rd acc 
+    = idoms ->
+  WF_idoms f idoms.
+Proof.
+  induction rd; simpl; intros; subst; auto.
+    remember 
+      (find_idom (dep_doms__nondep_doms (bound_fdef f) (dom_analyze f)) a) as R.
+    destruct R.
+      apply IHrd with (acc:=(l0, a) :: acc); auto.
+        admit.
+        apply WF_idoms_cons; auto.
+          admit.
+      apply IHrd with (acc:=acc); auto.
+        admit.
+Qed.
+
+Lemma compute_idoms__WF_idoms: forall f rd idoms,
+  reachablity_analysis f = Some rd ->
+  compute_idoms (dep_doms__nondep_doms (bound_fdef f) (dom_analyze f)) rd nil 
+    = idoms ->
+  WF_idoms f idoms.
+Proof.
+  intros.
+  apply compute_idoms__WF_idoms_aux in H0; auto.
+    apply WF_idoms_nil.
+Qed.
+
+Lemma init_create_pre_dtree_aux__WF_pre_dtree : forall f idoms pdt0 others 
+  pdt root rd,
+  getEntryLabel f = Some root ->
+  reachablity_analysis f = Some rd ->
+  compute_idoms (dep_doms__nondep_doms (bound_fdef f) (dom_analyze f)) rd nil 
+    = idoms ->
+  init_pre_dtree idoms root (List.remove eq_atom_dec root rd) 
+    = Some (pdt0, others) ->
+  create_pre_dtree_aux others idoms pdt0 = Some pdt ->
+  WF_pre_dtree f pdt.
+Proof.
+  intros.
+  eapply compute_idoms__WF_idoms in H1; eauto.
+  eapply create_pre_dtree_aux__WF_pre_dtree in H3; eauto.
+    eapply init_pre_dtree__disjoint; eauto.
+      apply remove_In.
+    eapply init_pre_dtree__WF_pre_dtree; eauto.
+Qed.
+
+Program Definition create_dtree (f: fdef) : option DTree :=
+match getEntryBlock f, reachablity_analysis f with
+| Some (block_intro root _ _ _), Some rd =>
+    let dt := dom_analyze f in
+    let b := bound_fdef f in
+    let idoms := compute_idoms (dep_doms__nondep_doms b dt) rd nil in
+    match init_pre_dtree idoms root (List.remove eq_atom_dec root rd) with
+    | None => None
+    | Some (pdt0, others) =>
+        match (create_pre_dtree_aux others idoms pdt0) with
+        | None => None
+        | Some pdt => 
+            tree2dtree 
+              (vertexes_of_pre_dtree pdt) (arcs_of_pre_dtree pdt)
+              (WF_pre_dtree_isa_tree f pdt _)
+        end
+    end
+| _, _ => None
+end.
+Next Obligation. 
+  eapply init_create_pre_dtree_aux__WF_pre_dtree; eauto.
+    clear - Heq_anonymous.
+    destruct f; simpl in *.
+    destruct b; simpl in *; inv Heq_anonymous. auto.
+Qed.
+
+Scheme dtree_rec2 := Induction for DTree Sort Set
+  with dtrees_rec2 := Induction for DTrees Sort Set.
+
+Definition dtree_mutrec P P' :=
+  fun h1 h2 h3 => 
+    (pair (@dtree_rec2 P P' h1 h2 h3) (@dtrees_rec2 P P' h1 h2 h3)).
+
+Definition dtree_insert__wf_dtree_prop (dt1:DTree) := 
+forall f a1 a0 dt2,
+  WF_dtree f dt1 ->
+  dtree_insert dt1 a1 a0 = ret dt2 ->
+  WF_dtree f dt2.
+
+Definition dtrees_insert__wf_dtrees_prop (dts1:DTrees) := 
+forall f root a1 a0 dts2,
+  WF_dtrees f root dts1 ->
+  dtrees_insert dts1 a1 a0 = ret dts2 ->
+  WF_dtrees f root dts2.
+
+Lemma dtree_insert__wf_dtree_mutrec :
+  (forall dt1, dtree_insert__wf_dtree_prop dt1) *
+  (forall dts1, dtrees_insert__wf_dtrees_prop dts1).
+Proof.
+  apply dtree_mutrec; 
+    unfold dtree_insert__wf_dtree_prop, dtrees_insert__wf_dtrees_prop;
+    simpl; intros.
+
+    inv H0.
+    destruct (id_dec a1 l0); subst.
+      inv H1.
+      apply WDT_node; simpl; auto.
+        admit.
+        apply WDT_cons; simpl; auto.
+          admit.
+          admit.
+          apply WDT_node; simpl; auto.
+            admit.
+            apply WDT_nil.
+       
+      remember (dtrees_insert d a1 a0) as R.
+      destruct R; inv H1. 
+        apply WDT_node; simpl; eauto.
+          admit.
+        
+    inv H0. auto.
+
+    remember (dtree_insert d a1 a0) as R.
+    destruct R; inv H2. 
+    remember (dtrees_insert d0 a1 a0) as R.
+    destruct R; inv H4. 
+    inv H1.
+    apply WDT_cons; simpl; eauto.
+      admit.
+      admit.
+Qed.
+
+Lemma dtree_insert__wf_dtree: forall f a1 a0 dt1 dt2,
+  WF_dtree f dt1 ->
+  dtree_insert dt1 a1 a0 = ret dt2 ->
+  WF_dtree f dt2.
+Proof.
+  induction dt1; simpl; intros.
+    destruct (id_dec a1 l0); subst.
+      inv H0.
+      inv H.
+      apply WDT_node; simpl; auto.
+        admit.
+        apply WDT_cons; simpl; auto.
+          admit.
+          admit.
+          apply WDT_node; simpl; auto.
+            admit.
+            apply WDT_nil.
+       
+      remember (dtrees_insert d a1 a0) as R.
+      destruct R.
+        inv H0. auto.
+
+
+Admitted.
+
+Lemma tree2dtree__wf_dtree: forall f vs es tree dt,
+  tree2dtree vs es tree = Some dt -> WF_dtree f dt.
+Proof.
+  induction tree; simpl; intros.
+    destruct r. inv H.
+    apply WDT_node.
+      admit.
+      simpl. fsetdec.
+      apply WDT_nil.
+
+    destruct f0. destruct n.
+    remember (tree2dtree v a tree) as R.
+    destruct R.
+      eapply dtree_insert__wf_dtree in H; eauto.
+      inv H.
+
+    apply IHtree in H; auto.
+Qed.
+
+(*
 Definition create_dtree (f: fdef) : option DTree :=
 match getEntryBlock f, reachablity_analysis f with
 | Some (block_intro root _ _ _), Some rd =>
@@ -366,6 +1181,7 @@ match getEntryBlock f, reachablity_analysis f with
       (List.remove eq_atom_dec root rd)
 | _, _ => None
 end.
+*)
 
 (*****************************)
 (*
